src/lib/poly/gemm/Old.Kuiper.Poly.GEMM.SHMem.fsti
@@ -1,0 +1,9 @@
+module Old.Kuiper.Poly.GEMM.SHMem
+
+#lang-pulse
+
+open Kuiper
+open Kuiper.Poly.GEMMGPU.Type
+
+inline_for_extraction noextract
+val mmcomb_gpu : tiled_matmulcomb_gpu_ty
